Update regex to v4.27.0-rc1

regex/Regex/Data/String.lean
@@ -5,85 +5,35 @@ def isWordChar (ch : Char) : Bool :=
 
 end Char
 
--- These theorems are backported from https://github.com/leanprover/lean4/pull/11289
-namespace String
-
-theorem Slice.Pos.le_of_not_lt {s : Slice} {p q : s.Pos} : ¬q < p → p ≤ q := by
-  simp [Slice.Pos.le_iff, Slice.Pos.lt_iff, Pos.Raw.le_iff, Pos.Raw.lt_iff]
-
-theorem Slice.Pos.ne_endPos_of_lt {s : Slice} {p q : s.Pos} : p < q → p ≠ s.endPos := by
-  have := q.isValidForSlice.le_utf8ByteSize
-  simp [lt_iff, Pos.ext_iff, Pos.Raw.lt_iff, Pos.Raw.ext_iff]
-  omega
-
-theorem Slice.Pos.next_le_of_lt {s : Slice} {p q : s.Pos} {h} : p < q → p.next h ≤ q := by
-  -- Things like this will become a lot simpler once we have the `Splits` machinery developed,
-  -- but this is `String.Basic`, so we have to suffer a little.
-  refine fun hpq => le_of_not_lt (fun hq => ?_)
-  have := q.isUTF8FirstByte_byte (h := ne_endPos_of_lt hq)
-  rw [byte, getUTF8Byte, String.getUTF8Byte] at this
-  simp only [Pos.Raw.byteIdx_offsetBy] at this
-  have h₁ : q.offset.byteIdx = p.offset.byteIdx + (q.offset.byteIdx - p.offset.byteIdx) := by
-    simp [lt_iff, Pos.Raw.lt_iff] at hpq
-    omega
-  have h₂ : q.offset.byteIdx - p.offset.byteIdx < (p.get h).utf8Size := by
-    simp [lt_iff, Pos.Raw.lt_iff] at hq
-    omega
-  conv at this => congr; arg 2; rw [h₁, ← Nat.add_assoc]
-  rw [← ByteArray.getElem_extract (start := s.startInclusive.offset.byteIdx + p.offset.byteIdx)
-    (stop := s.startInclusive.offset.byteIdx + p.offset.byteIdx + (p.get h).utf8Size)] at this
-  · simp only [← utf8Encode_get_eq_extract, List.utf8Encode_singleton] at this
-    have h₃ := List.getElem_toByteArray (l := utf8EncodeChar (p.get h))
-      (i := q.offset.byteIdx - p.offset.byteIdx) (h := by simpa)
-    rw [h₃, UInt8.isUTF8FirstByte_getElem_utf8EncodeChar] at this
-    simp only [lt_iff, Pos.Raw.lt_iff] at hpq
-    omega
-  · simp only [ByteArray.size_extract, size_bytes]
-    rw [Nat.min_eq_left]
-    · omega
-    · have := (p.next h).str.isValid.le_utf8ByteSize
-      simpa [Nat.add_assoc] using this
-
-theorem Slice.Pos.ofSlice_le_iff {s : String} {p : s.toSlice.Pos} {q : s.ValidPos} :
-    p.ofSlice ≤ q ↔ p ≤ q.toSlice := Iff.rfl
-
-@[simp]
-theorem ValidPos.toSlice_lt_toSlice_iff {s : String} {p q : s.ValidPos} :
-    p.toSlice < q.toSlice ↔ p < q := Iff.rfl
-
-theorem ValidPos.next_le_of_lt {s : String} {p q : s.ValidPos} {h} : p < q → p.next h ≤ q := by
-  rw [next, Slice.Pos.ofSlice_le_iff, ← ValidPos.toSlice_lt_toSlice_iff]
-  exact Slice.Pos.next_le_of_lt
-
-end String
-
-namespace String.ValidPos
+namespace Regex.Data.String
 
 open Char
+open _root_.String (Pos)
 
 variable {s : String}
 
-def isCurrWord (p : ValidPos s) : Bool :=
-  if h : p ≠ s.endValidPos then
+def isCurrWord (p : Pos s) : Bool :=
+  if h : p ≠ s.endPos then
     isWordChar (p.get h)
   else
     false
 
-def isPrevWord (p : ValidPos s) : Bool :=
-  if h : p ≠ s.startValidPos then
+def isPrevWord (p : Pos s) : Bool :=
+  if h : p ≠ s.startPos then
     isWordChar ((p.prev h).get (by simp))
   else
     false
 
-def isAtWordBoundary (p : ValidPos s) : Bool :=
+def isAtWordBoundary (p : Pos s) : Bool :=
   isCurrWord p != isPrevWord p
 
-def isAtNonWordBoundary (p : ValidPos s) : Bool :=
+def isAtNonWordBoundary (p : Pos s) : Bool :=
   isCurrWord p == isPrevWord p
 
+-- A simpler version of `String.Pos.find` that's easier to prove the correctness.
 @[specialize]
-def find (pos : ValidPos s) (p : Char → Bool) :=
-  if hn : pos = s.endValidPos then
+def find (pos : Pos s) (p : Char → Bool) :=
+  if hn : pos = s.endPos then
     pos
   else if p (pos.get hn) then
     pos
@@ -91,51 +41,51 @@ def find (pos : ValidPos s) (p : Char → Bool) :=
     find (pos.next hn) p
 termination_by pos
 
-end String.ValidPos
+end Regex.Data.String
 
-namespace String.ValidPos
+namespace String.Pos
 
-theorem ne_endValidPos_of_lt {s : String} {pos pos' : ValidPos s} (lt : pos < pos') : pos ≠ s.endValidPos := by
+theorem ne_endPos_of_lt {s : String} {pos pos' : Pos s} (lt : pos < pos') : pos ≠ s.endPos := by
   intro eq
-  have : pos'.offset ≤ s.endValidPos.offset := pos'.isValid.le_rawEndPos
+  have : pos'.offset ≤ s.endPos.offset := pos'.isValid.le_rawEndPos
   exact Nat.not_le_of_lt (eq ▸ lt) this
 
 @[grind ., simp]
-theorem ne_next {s : String} {pos : ValidPos s} {ne : pos ≠ s.endValidPos} : pos ≠ pos.next ne := by
+theorem ne_next {s : String} {pos : Pos s} {ne : pos ≠ s.endPos} : pos ≠ pos.next ne := by
   intro eq
   have : pos.next ne < pos.next ne := eq ▸ pos.lt_next
   exact (Nat.lt_irrefl _ this).elim
 
-def posRevInduction.{u} {s : String} {motive : ValidPos s → Sort u}
-  (endValidPos : motive s.endValidPos)
-  (next : ∀ p : ValidPos s, (h : p ≠ s.endValidPos) → motive (p.next h) → motive p)
-  (p : ValidPos s) : motive p :=
-  if h : p = s.endValidPos then
-    h ▸ endValidPos
+def posRevInduction.{u} {s : String} {motive : Pos s → Sort u}
+  (endPos : motive s.endPos)
+  (next : ∀ p : Pos s, (h : p ≠ s.endPos) → motive (p.next h) → motive p)
+  (p : Pos s) : motive p :=
+  if h : p = s.endPos then
+    h ▸ endPos
   else
-    next p h (posRevInduction endValidPos next (p.next h))
+    next p h (posRevInduction endPos next (p.next h))
   termination_by p
 
-theorem splits_of_next {s l r : String} {p : ValidPos s} {h : p ≠ s.endValidPos}
+theorem splits_of_next {s l r : String} {p : Pos s} {h : p ≠ s.endPos}
   (sp : (p.next h).Splits (l ++ singleton (p.get h)) r) : p.Splits l (singleton (p.get h) ++ r) where
   eq_append := by simp only [sp.eq_append, String.append_assoc]
-  offset_eq_rawEndPos := by simpa [offset_next, Pos.Raw.ext_iff] using sp.offset_eq_rawEndPos
+  offset_eq_rawEndPos := by simpa [Pos.next, Pos.Raw.ext_iff] using sp.offset_eq_rawEndPos
 
-theorem splits_get_singleton {s l r : String} {c : Char} {p : ValidPos s} (sp : p.Splits l (singleton c ++ r)) :
-  p.get sp.ne_endValidPos_of_singleton = c := by
-  obtain ⟨r', h⟩ := sp.exists_eq_singleton_append sp.ne_endValidPos_of_singleton
+theorem splits_get_singleton {s l r : String} {c : Char} {p : Pos s} (sp : p.Splits l (singleton c ++ r)) :
+  p.get sp.ne_endPos_of_singleton = c := by
+  obtain ⟨r', h⟩ := sp.exists_eq_singleton_append sp.ne_endPos_of_singleton
   simp only [singleton_append_inj] at h
   exact h.1.symm
 
-theorem lt_or_eq_of_le {s : String} {p p' : ValidPos s} (le : p ≤ p') : p < p' ∨ p = p' := by
+theorem lt_or_eq_of_le {s : String} {p p' : Pos s} (le : p ≤ p') : p < p' ∨ p = p' := by
   cases Nat.lt_or_eq_of_le le with
   | inl lt => exact .inl lt
-  | inr eq => exact .inr (by simp [ValidPos.ext_iff, Pos.Raw.ext_iff, eq])
+  | inr eq => exact .inr (by simp [Pos.ext_iff, Pos.Raw.ext_iff, eq])
 
-theorem Splits.exists_eq_append_left_of_lt {s l r : String} {p p' : ValidPos s} (sp : p.Splits l r) (lt : p' < p) :
+theorem Splits.exists_eq_append_left_of_lt {s l r : String} {p p' : Pos s} (sp : p.Splits l r) (lt : p' < p) :
   ∃ l₁ l₂, l = l₁ ++ l₂ ∧ p'.Splits l₁ (l₂ ++ r) := by
   induction p' using posRevInduction with
-  | endValidPos => exact (Nat.not_lt_of_le p.isValid.le_rawEndPos lt).elim
+  | endPos => exact (Nat.not_lt_of_le p.isValid.le_rawEndPos lt).elim
   | next p' h ih =>
     have : p'.next h < p ∨ p'.next h = p := lt_or_eq_of_le (next_le_of_lt lt)
     cases this with
@@ -149,47 +99,45 @@ theorem Splits.exists_eq_append_left_of_lt {s l r : String} {p p' : ValidPos s} 
       obtain ⟨l, rfl⟩ := sp.exists_eq_append_singleton
       exact ⟨l, singleton (p'.get h), rfl, splits_of_next sp⟩
 
-theorem next_inj {s} {pos pos' : ValidPos s} {h : pos ≠ s.endValidPos} {h' : pos' ≠ s.endValidPos}
+theorem next_inj {s} {pos pos' : Pos s} {h : pos ≠ s.endPos} {h' : pos' ≠ s.endPos}
   (eq : pos.next h = pos'.next h') :
   pos = pos' := by
   have eq' := (pos.splits_next h).eq_left (eq ▸ pos'.splits_next h')
   simp only [append_singleton, push_inj] at eq'
-  exact ValidPos.ext (Eq.trans (eq'.1 ▸ pos.splits.offset_eq_rawEndPos) (pos'.splits.offset_eq_rawEndPos).symm)
+  exact Pos.ext (Eq.trans (eq'.1 ▸ pos.splits.offset_eq_rawEndPos) (pos'.splits.offset_eq_rawEndPos).symm)
 
-theorem lt_of_le_of_ne {s} {pos pos' : ValidPos s} (le : pos ≤ pos') (ne : pos ≠ pos') : pos < pos' :=
-  Nat.lt_of_le_of_ne le (by simpa [ValidPos.ext_iff, Pos.Raw.ext_iff] using ne)
+theorem le_of_lt_next {s} {pos pos' : Pos s} {h' : pos' ≠ s.endPos} (lt : pos < pos'.next h') : pos ≤ pos' :=
+  Decidable.by_contra (fun nle => Nat.not_lt_of_le (Pos.next_le_of_lt (Nat.lt_of_not_le nle)) lt)
 
-theorem le_of_lt_next {s} {pos pos' : ValidPos s} {h' : pos' ≠ s.endValidPos} (lt : pos < pos'.next h') : pos ≤ pos' :=
-  Decidable.by_contra (fun nle => Nat.not_lt_of_le (ValidPos.next_le_of_lt (Nat.lt_of_not_le nle)) lt)
-
-theorem le_or_eq_of_le_next {s} {pos pos' : ValidPos s} {h' : pos' ≠ s.endValidPos} (le : pos ≤ pos'.next h') :
+theorem le_or_eq_of_le_next {s} {pos pos' : Pos s} {h' : pos' ≠ s.endPos} (le : pos ≤ pos'.next h') :
   pos ≤ pos' ∨ pos = pos'.next h' :=
   Decidable.byCases
     (fun (eq : pos = pos'.next h') => .inr eq)
     (fun (ne : pos ≠ pos'.next h') => .inl (le_of_lt_next (lt_of_le_of_ne le ne)))
 
-theorem le_next_iff {s} {pos pos' : ValidPos s} {h' : pos' ≠ s.endValidPos} :
+theorem le_next_iff {s} {pos pos' : Pos s} {h' : pos' ≠ s.endPos} :
   pos ≤ pos'.next h' ↔ pos ≤ pos' ∨ pos = pos'.next h' := by
   refine ⟨le_or_eq_of_le_next, ?_⟩
   intro h
   cases h with
-  | inl le => exact le_trans le (le_of_lt pos'.lt_next)
-  | inr eq => exact eq ▸ le_refl _
+  | inl le => exact Nat.le_trans le (Nat.le_of_lt pos'.lt_next)
+  | inr eq => exact eq ▸ Nat.le_refl _
 
-theorem lt_next_iff {s} {pos pos' : ValidPos s} {h' : pos' ≠ s.endValidPos} : pos < pos'.next h' ↔ pos ≤ pos' :=
+theorem lt_next_iff {s} {pos pos' : Pos s} {h' : pos' ≠ s.endPos} : pos < pos'.next h' ↔ pos ≤ pos' :=
   ⟨le_of_lt_next, fun le => Nat.lt_of_le_of_lt le pos'.lt_next⟩
 
-theorem le_iff_lt_or_eq {s} {pos pos' : ValidPos s} : pos ≤ pos' ↔ pos < pos' ∨ pos = pos' :=
-  Iff.trans Nat.le_iff_lt_or_eq (or_congr Iff.rfl (by simp [ValidPos.ext_iff, Pos.Raw.ext_iff]))
+theorem le_iff_lt_or_eq {s} {pos pos' : Pos s} : pos ≤ pos' ↔ pos < pos' ∨ pos = pos' :=
+  Iff.trans Nat.le_iff_lt_or_eq (or_congr Iff.rfl (by simp [Pos.ext_iff, Pos.Raw.ext_iff]))
 
-theorem lt_next_iff_lt_or_eq {s} {pos pos' : ValidPos s} (h' : pos' ≠ s.endValidPos) :
+theorem lt_next_iff_lt_or_eq {s} {pos pos' : Pos s} (h' : pos' ≠ s.endPos) :
   pos < pos'.next h' ↔ pos < pos' ∨ pos = pos' :=
   lt_next_iff.trans le_iff_lt_or_eq
 
-end String.ValidPos
+end String.Pos
 
 namespace String
 
+-- TODO: rename to `PosPlusOne`
 @[ext]
 structure ValidPosPlusOne (s : String) where
   offset : Pos.Raw
@@ -202,7 +150,7 @@ variable {s : String}
 
 -- Doesn't seem to work at the moment
 @[match_pattern]
-def validPos (p : ValidPos s) : ValidPosPlusOne s :=
+def validPos (p : Pos s) : ValidPosPlusOne s :=
   ⟨p.offset, .inl p.isValid⟩
 
 @[match_pattern]
@@ -211,7 +159,7 @@ def sentinel (s : String) : ValidPosPlusOne s :=
 
 @[elab_as_elim, cases_eliminator]
 def rec'.{u} {motive : ValidPosPlusOne s → Sort u}
-  (validPos : (p : ValidPos s) → motive (validPos p))
+  (validPos : (p : Pos s) → motive (validPos p))
   (sentinel : motive (sentinel s))
   (p : ValidPosPlusOne s) : motive p :=
   if h : p.offset = s.rawEndPos.offsetBy ⟨1⟩ then
@@ -225,7 +173,7 @@ def rec'.{u} {motive : ValidPosPlusOne s → Sort u}
       | inr h => contradiction
     validPos ⟨p.offset, h'⟩
 
-instance : Inhabited (ValidPosPlusOne s) := ⟨.validPos s.startValidPos⟩
+instance : Inhabited (ValidPosPlusOne s) := ⟨.validPos s.startPos⟩
 
 @[inline]
 def isValid (p : ValidPosPlusOne s) : Bool :=
@@ -248,7 +196,7 @@ theorem isValid_iff_isValid (p : ValidPosPlusOne s) : p.isValid ↔ p.offset.IsV
       grind
     simpa [isValid, h]
 
-def asValidPos (p : ValidPosPlusOne s) (h : p.isValid) : ValidPos s :=
+def asValidPos (p : ValidPosPlusOne s) (h : p.isValid) : Pos s :=
   ⟨p.offset, p.isValid_iff_isValid.mp h⟩
 
 def lt (p₁ p₂ : ValidPosPlusOne s) : Prop :=
@@ -264,7 +212,7 @@ instance {s : String} (p₁ p₂ : ValidPosPlusOne s) : Decidable (p₁ < p₂) 
 
 def next (p : ValidPosPlusOne s) (h : p.isValid) : ValidPosPlusOne s :=
   let vp := p.asValidPos h
-  if h' : vp ≠ s.endValidPos then
+  if h' : vp ≠ s.endPos then
     .validPos (vp.next h')
   else
     .sentinel s
@@ -275,7 +223,7 @@ theorem lt_sentinel_of_valid {p : ValidPosPlusOne s} (h : p.isValid) : p < .sent
 @[simp, grind →]
 theorem lt_next (p : ValidPosPlusOne s) (h : p.isValid) : p < p.next h := by
   fun_cases next
-  next vp ne => exact ValidPos.lt_next (p.asValidPos h) (h := ne)
+  next vp ne => exact Pos.lt_next (p := p.asValidPos h) (h := ne)
   next => exact lt_sentinel_of_valid h
 
 def remainingBytes (p : ValidPosPlusOne s) : Nat :=
@@ -306,7 +254,7 @@ theorem le_iff {p₁ p₂ : ValidPosPlusOne s} : p₁ ≤ p₂ ↔ p₁.offset �
   Iff.rfl
 
 @[simp, grind =]
-theorem validPos_le_validPos_iff {p₁ p₂ : ValidPos s} : ValidPosPlusOne.validPos p₁ ≤ ValidPosPlusOne.validPos p₂ ↔ p₁ ≤ p₂ :=
+theorem validPos_le_validPos_iff {p₁ p₂ : Pos s} : ValidPosPlusOne.validPos p₁ ≤ ValidPosPlusOne.validPos p₂ ↔ p₁ ≤ p₂ :=
   Iff.rfl
 
 instance {s : String} (p₁ p₂ : ValidPosPlusOne s) : Decidable (p₁ ≤ p₂) :=
@@ -323,9 +271,9 @@ theorem isValid_of_isValid_of_le {p₁ p₂ : ValidPosPlusOne s} (h : p₂.isVal
     grind
 
 @[grind .]
-theorem validPos_inj {p₁ p₂ : ValidPos s} (h : ValidPosPlusOne.validPos p₁ = ValidPosPlusOne.validPos p₂) : p₁ = p₂ := by
+theorem validPos_inj {p₁ p₂ : Pos s} (h : ValidPosPlusOne.validPos p₁ = ValidPosPlusOne.validPos p₂) : p₁ = p₂ := by
   simp only [validPos, ValidPosPlusOne.mk.injEq] at h
-  exact ValidPos.ext h
+  exact Pos.ext h
 
 def or (p₁ p₂ : ValidPosPlusOne s) : ValidPosPlusOne s :=
   if p₁.isValid then
@@ -357,12 +305,13 @@ theorem or_not_valid {p₁ p₂ : ValidPosPlusOne s} (h : ¬p₁.isValid) : p₁
   simp [or, h]
 
 @[simp, grind =]
-theorem isValid_validPos {p : ValidPos s} : (ValidPosPlusOne.validPos p).isValid = true :=
+theorem isValid_validPos {p : Pos s} : (ValidPosPlusOne.validPos p).isValid = true :=
   (isValid_iff_isValid (.validPos p)).mpr p.isValid
 
 @[simp, grind =]
 theorem not_isValid_sentinel {s : String} : (ValidPosPlusOne.sentinel s).isValid = false := by
   simp [sentinel, isValid]
+
 @[simp, grind =]
 theorem sentinel_or {p₁ p₂ : ValidPosPlusOne s} (h : p₁ = .sentinel s) : p₁.or p₂ = p₂ := by
   grind
@@ -378,7 +327,7 @@ theorem or_sentinel {p₁ p₂ : ValidPosPlusOne s} (h : p₂ = .sentinel s) : p
   | sentinel => simp [h]
 
 @[grind .]
-theorem validPos_ne_sentinel {p : ValidPos s} : ValidPosPlusOne.validPos p ≠ ValidPosPlusOne.sentinel s := by
+theorem validPos_ne_sentinel {p : Pos s} : ValidPosPlusOne.validPos p ≠ ValidPosPlusOne.sentinel s := by
   intro eq
   have : isValid (.validPos p) = isValid (.sentinel s) := by grind
   simp at this
@@ -390,7 +339,7 @@ theorem or_self {p : ValidPosPlusOne s} : p.or p = p := by
   | sentinel => simp
 
 @[simp, grind =]
-theorem asValidPos_validPos {p : ValidPos s} : (ValidPosPlusOne.validPos p).asValidPos (by grind) = p := rfl
+theorem asValidPos_validPos {p : Pos s} : (ValidPosPlusOne.validPos p).asValidPos (by grind) = p := rfl
 
 @[simp, grind =]
 theorem validPos_asValidPos {p : ValidPosPlusOne s} {h : p.isValid} : (ValidPosPlusOne.validPos (p.asValidPos h)) = p := rfl
@@ -398,6 +347,6 @@ theorem validPos_asValidPos {p : ValidPosPlusOne s} {h : p.isValid} : (ValidPosP
 end ValidPosPlusOne
 
 def startValidPosPlusOne (s : String) : ValidPosPlusOne s :=
-  .validPos s.startValidPos
+  .validPos s.startPos
 
 end String
