regex/Regex/Syntax/Parser/Combinators/Rel.lean
@@ -1,16 +1,16 @@
 set_option autoImplicit false
 
-open String (ValidPos)
+open String (Pos)
 
 namespace Regex.Syntax.Parser.Combinators
 
 variable {s : String}
 
-def Rel.LE (p' p : ValidPos s) : Prop := p ≤ p'
+def Rel.LE (p' p : Pos s) : Prop := p ≤ p'
 
-def Rel.LT (p' p : ValidPos s) : Prop := p < p'
+def Rel.LT (p' p : Pos s) : Prop := p < p'
 
-def Rel (strict : Bool) : ValidPos s → ValidPos s → Prop :=
+def Rel (strict : Bool) : Pos s → Pos s → Prop :=
   if strict then Rel.LT else Rel.LE
 
 namespace Rel
@@ -27,17 +27,17 @@ instance : Trans (@Rel.LT s) (@Rel.LE s) (@Rel.LT s) where
 instance : Trans (@Rel.LT s) (@Rel.LT s) (@Rel.LT s) where
   trans h h' := Nat.lt_trans h' h
 
-def imp {strict₁ strict₂ : Bool} {p' p : ValidPos s} (h : strict₂ → strict₁) (rel : Rel strict₁ p' p) : Rel strict₂ p' p :=
+def imp {strict₁ strict₂ : Bool} {p' p : Pos s} (h : strict₂ → strict₁) (rel : Rel strict₁ p' p) : Rel strict₂ p' p :=
   match strict₁, strict₂ with
   | false, false => rel
   | false, true => by simp at h
   | true, false => Nat.le_of_lt rel
   | true, true => rel
 
-def weaken {strict : Bool} {p' p : ValidPos s} (rel : Rel strict p' p) : Rel false p' p :=
+def weaken {strict : Bool} {p' p : Pos s} (rel : Rel strict p' p) : Rel false p' p :=
   rel.imp (by simp)
 
-def transOr {strict₁ strict₂ : Bool} {p p' p'' : ValidPos s} (h : Rel strict₁ p p') (h' : Rel strict₂ p' p'') : Rel (strict₁ || strict₂) p p'' := by
+def transOr {strict₁ strict₂ : Bool} {p p' p'' : Pos s} (h : Rel strict₁ p p') (h' : Rel strict₂ p' p'') : Rel (strict₁ || strict₂) p p'' := by
   match strict₁, strict₂ with
   | false, false =>
     simp [Rel] at *
@@ -52,7 +52,7 @@ def transOr {strict₁ strict₂ : Bool} {p p' p'' : ValidPos s} (h : Rel strict
     simp [Rel] at *
     exact Trans.trans h h'
 
-def trans {strict : Bool} {p p' p'' : ValidPos s} (h : Rel strict p p') (h' : Rel strict p' p'') : Rel strict p p'' :=
+def trans {strict : Bool} {p p' p'' : Pos s} (h : Rel strict p p') (h' : Rel strict p' p'') : Rel strict p p'' :=
   (Bool.or_self strict) ▸ transOr h h'
 
 instance {strict₁ strict₂ : Bool} : Trans (@Rel s strict₁) (@Rel s strict₂) (@Rel s (strict₁ || strict₂)) where
