regex/Regex/Syntax/Parser/Combinators/Result.lean
@@ -2,66 +2,66 @@ import Regex.Syntax.Parser.Combinators.Rel
 
 set_option autoImplicit false
 
-open String (ValidPos)
+open String (Pos)
 
 namespace Regex.Syntax.Parser.Combinators
 
 variable {s : String}
 
-inductive Result (strict : Bool) (p : ValidPos s) (ε α : Type) where
-  | ok : α → (p' : ValidPos s) → Rel strict p' p → Result strict p ε α
+inductive Result (strict : Bool) (p : Pos s) (ε α : Type) where
+  | ok : α → (p' : Pos s) → Rel strict p' p → Result strict p ε α
   | error : ε → Result strict p ε α
   | fatal : ε → Result strict p ε α
 
 namespace Result
 
-abbrev LE (p : ValidPos s) (ε α : Type) := Result false p ε α
+abbrev LE (p : Pos s) (ε α : Type) := Result false p ε α
 
-abbrev LT (p : ValidPos s) (ε α : Type) := Result true p ε α
+abbrev LT (p : Pos s) (ε α : Type) := Result true p ε α
 
 @[inline]
-def imp {strict₁ strict₂ : Bool} {p : ValidPos s} {ε α} (h : strict₂ → strict₁) : Result strict₁ p ε α → Result strict₂ p ε α
+def imp {strict₁ strict₂ : Bool} {p : Pos s} {ε α} (h : strict₂ → strict₁) : Result strict₁ p ε α → Result strict₂ p ε α
   | .ok a pos' h' => .ok a pos' (h'.imp h)
   | .error e => .error e
   | .fatal e => .fatal e
 
 @[inline]
-def transOr {strict₁ strict₂ : Bool} {p p' : ValidPos s} {ε α} (h : Rel strict₂ p' p) : Result strict₁ p' ε α → Result (strict₁ || strict₂) p ε α
+def transOr {strict₁ strict₂ : Bool} {p p' : Pos s} {ε α} (h : Rel strict₂ p' p) : Result strict₁ p' ε α → Result (strict₁ || strict₂) p ε α
   | .ok a pos'' h' => .ok a pos'' (Rel.transOr h' h)
   | .error e => .error e
   | .fatal e => .fatal e
 
 @[inline]
-def trans {strict : Bool} {p p' : ValidPos s} {ε α} (h : Rel strict p p') : Result strict p ε α → Result strict p' ε α
+def trans {strict : Bool} {p p' : Pos s} {ε α} (h : Rel strict p p') : Result strict p ε α → Result strict p' ε α
   | .ok a pos'' h' => .ok a pos'' (Rel.trans h' h)
   | .error e => .error e
   | .fatal e => .fatal e
 
 @[inline]
-def cast {strict₁ strict₂ : Bool} {p : ValidPos s} {ε α} (h : strict₁ = strict₂) (res : Result strict₁ p ε α) : Result strict₂ p ε α :=
+def cast {strict₁ strict₂ : Bool} {p : Pos s} {ε α} (h : strict₁ = strict₂) (res : Result strict₁ p ε α) : Result strict₂ p ε α :=
   res.imp (by simp [h])
 
 @[inline]
-def weaken {strict : Bool} {p : ValidPos s} {ε α} (res : Result strict p ε α) : Result false p ε α :=
+def weaken {strict : Bool} {p : Pos s} {ε α} (res : Result strict p ε α) : Result false p ε α :=
   res.imp (by simp)
 
 @[inline]
-def toExcept {strict : Bool} {p : ValidPos s} {ε α} (res : Result strict p ε α) : Except ε α :=
+def toExcept {strict : Bool} {p : Pos s} {ε α} (res : Result strict p ε α) : Except ε α :=
   match res with
   | .ok a _ _ => .ok a
   | .error e => .error e
   | .fatal e => .error e
 
 @[inline]
-def opt {strict : Bool} {p : ValidPos s} {ε α} : Result strict p ε α → Result false p ε (Option α)
+def opt {strict : Bool} {p : Pos s} {ε α} : Result strict p ε α → Result false p ε (Option α)
   | .ok a p' h => .ok (.some a) p' h.weaken
   | .error _ => .ok .none p (Nat.le_refl _)
   | .fatal e => .fatal e
 
 @[inline]
-def complete {strict : Bool} {p : ValidPos s} {ε α} (expectedEof : ε) : Result strict p ε α → Result strict p ε α
+def complete {strict : Bool} {p : Pos s} {ε α} (expectedEof : ε) : Result strict p ε α → Result strict p ε α
   | .ok a p' h =>
-    if p' == s.endValidPos then
+    if p' == s.endPos then
       .ok a p' h
     else
       .error expectedEof
@@ -69,13 +69,13 @@ def complete {strict : Bool} {p : ValidPos s} {ε α} (expectedEof : ε) : Resul
   | .fatal e => .fatal e
 
 @[inline]
-def commit {strict : Bool} {p : ValidPos s} {ε α} : Result strict p ε α → Result strict p ε α
+def commit {strict : Bool} {p : Pos s} {ε α} : Result strict p ε α → Result strict p ε α
   | .ok a p' h => .ok a p' h
   | .error e => .fatal e
   | .fatal e => .fatal e
 
 @[inline]
-def guard {strict : Bool} {p : ValidPos s} {ε α β} (f : α → Except ε β) : Result strict p ε α → Result strict p ε β
+def guard {strict : Bool} {p : Pos s} {ε α β} (f : α → Except ε β) : Result strict p ε α → Result strict p ε β
   | .ok a p' h =>
     match f a with
     | .ok b => .ok b p' h
@@ -84,17 +84,17 @@ def guard {strict : Bool} {p : ValidPos s} {ε α β} (f : α → Except ε β) 
   | .fatal e => .fatal e
 
 @[inline]
-def map' {strict : Bool} {p : ValidPos s} {ε α β} (f : α → (p' : ValidPos s) → Rel strict p' p → β) : Result strict p ε α → Result strict p ε β
+def map' {strict : Bool} {p : Pos s} {ε α β} (f : α → (p' : Pos s) → Rel strict p' p → β) : Result strict p ε α → Result strict p ε β
   | .ok a p' h => .ok (f a p' h) p' h
   | .error e => .error e
   | .fatal e => .fatal e
 
 @[inline]
-def map {strict : Bool} {p : ValidPos s} {ε α β} (f : α → β) : Result strict p ε α → Result strict p ε β :=
+def map {strict : Bool} {p : Pos s} {ε α β} (f : α → β) : Result strict p ε α → Result strict p ε β :=
   map' fun a _ _ => f a
 
 @[inline]
-def seq {strict : Bool} {p : ValidPos s} {ε α β} (mf : Result strict p ε (α → β)) (mx : Unit → Result strict p ε α) : Result strict p ε β :=
+def seq {strict : Bool} {p : Pos s} {ε α β} (mf : Result strict p ε (α → β)) (mx : Unit → Result strict p ε α) : Result strict p ε β :=
   match mf with
   | .ok f _ _ =>
     match mx () with
@@ -105,7 +105,7 @@ def seq {strict : Bool} {p : ValidPos s} {ε α β} (mf : Result strict p ε (α
   | .fatal e => .fatal e
 
 @[inline]
-def seqLeft {strict : Bool} {p : ValidPos s} {ε α β} (mx : Result strict p ε α) (my : Unit → Result strict p ε β) : Result strict p ε α :=
+def seqLeft {strict : Bool} {p : Pos s} {ε α β} (mx : Result strict p ε α) (my : Unit → Result strict p ε β) : Result strict p ε α :=
   match mx with
   | .ok a _ _ =>
     match my () with
@@ -116,7 +116,7 @@ def seqLeft {strict : Bool} {p : ValidPos s} {ε α β} (mx : Result strict p ε
   | .fatal e => .fatal e
 
 @[inline]
-def seqRight {strict : Bool} {p : ValidPos s} {ε α β} (mx : Result strict p ε α) (my : Unit → Result strict p ε β) : Result strict p ε β :=
+def seqRight {strict : Bool} {p : Pos s} {ε α β} (mx : Result strict p ε α) (my : Unit → Result strict p ε β) : Result strict p ε β :=
   match mx with
   | .ok _ _ _ =>
     match my () with
@@ -127,84 +127,84 @@ def seqRight {strict : Bool} {p : ValidPos s} {ε α β} (mx : Result strict p �
   | .fatal e => .fatal e
 
 @[inline]
-def hOrElse {strict₁ strict₂ : Bool} {p : ValidPos s} {ε α} (mx : Result strict₁ p ε α) (my : Unit → Result strict₂ p ε α) : Result (strict₁ && strict₂) p ε α :=
+def hOrElse {strict₁ strict₂ : Bool} {p : Pos s} {ε α} (mx : Result strict₁ p ε α) (my : Unit → Result strict₂ p ε α) : Result (strict₁ && strict₂) p ε α :=
   match mx with
   | .ok a p' h => .ok a p' (h.imp (by simp_all))
   | .error _ => (my ()).imp (by simp)
   | .fatal e => .fatal e
 
 @[inline]
-def orElse {strict : Bool} {p : ValidPos s} {ε α} : Result strict p ε α → (Unit → Result strict p ε α) → Result strict p ε α
+def orElse {strict : Bool} {p : Pos s} {ε α} : Result strict p ε α → (Unit → Result strict p ε α) → Result strict p ε α
   | .ok a p' h, _ => .ok a p' h
   | .error _, b => b ()
   | .fatal e, _ => .fatal e
 
 @[inline]
-def throw {strict : Bool} {p : ValidPos s} {ε α} (e : ε) : Result strict p ε α := .error e
+def throw {strict : Bool} {p : Pos s} {ε α} (e : ε) : Result strict p ε α := .error e
 
 @[inline]
-def tryCatch {strict : Bool} {p : ValidPos s} {ε α} (mx : Result strict p ε α) (handle : ε → Result strict p ε α) : Result strict p ε α :=
+def tryCatch {strict : Bool} {p : Pos s} {ε α} (mx : Result strict p ε α) (handle : ε → Result strict p ε α) : Result strict p ε α :=
   match mx with
   | .ok a p' h => .ok a p' h
   | .error e => handle e
   | .fatal e => .fatal e
 
 @[inline]
-def bind' {strict₁ strict₂ : Bool} {p : ValidPos s} {ε α β} (mx : Result strict₁ p ε α) (f : α → (p' : ValidPos s) → Rel strict₁ p' p → Result strict₂ p' ε β) : Result (strict₁ || strict₂) p ε β :=
+def bind' {strict₁ strict₂ : Bool} {p : Pos s} {ε α β} (mx : Result strict₁ p ε α) (f : α → (p' : Pos s) → Rel strict₁ p' p → Result strict₂ p' ε β) : Result (strict₁ || strict₂) p ε β :=
   match mx with
   | .ok a p' h => (f a p' h).transOr h |>.cast (Bool.or_comm _ _)
   | .error e => .error e
   | .fatal e => .fatal e
 
 @[inline]
-def bind {strict : Bool} {p : ValidPos s} {ε α β} (mx : Result strict p ε α) (f : α → Result strict p ε β) : Result strict p ε β :=
+def bind {strict : Bool} {p : Pos s} {ε α β} (mx : Result strict p ε α) (f : α → Result strict p ε β) : Result strict p ε β :=
   match mx with
   | .ok a _ _ => f a
   | .error e => .error e
   | .fatal e => .fatal e
 
 @[inline]
-def pure {p : ValidPos s} {ε α} (a : α) : LE p ε α := .ok a p (Nat.le_refl _)
+def pure {p : Pos s} {ε α} (a : α) : LE p ε α := .ok a p (Nat.le_refl _)
 
 @[inline]
-instance {strict : Bool} {p : ValidPos s} {ε} : Functor (Result strict p ε) where
+instance {strict : Bool} {p : Pos s} {ε} : Functor (Result strict p ε) where
   map := map
 
 @[inline]
-instance {strict : Bool} {p : ValidPos s} {ε} : Seq (Result strict p ε) where
+instance {strict : Bool} {p : Pos s} {ε} : Seq (Result strict p ε) where
   seq := seq
 
 @[inline]
-instance {strict : Bool} {p : ValidPos s} {ε} : SeqLeft (Result strict p ε) where
+instance {strict : Bool} {p : Pos s} {ε} : SeqLeft (Result strict p ε) where
 seqLeft := seqLeft
 
 @[inline]
-instance {strict : Bool} {p : ValidPos s} {ε} : SeqRight (Result strict p ε) where
+instance {strict : Bool} {p : Pos s} {ε} : SeqRight (Result strict p ε) where
   seqRight := seqRight
 
 @[inline]
-instance {strict₁ strict₂ : Bool} {p : ValidPos s} {ε α} : HOrElse (Result strict₁ p ε α) (Result strict₂ p ε α) (Result (strict₁ && strict₂) p ε α) where
+instance {strict₁ strict₂ : Bool} {p : Pos s} {ε α} : HOrElse (Result strict₁ p ε α) (Result strict₂ p ε α) (Result (strict₁ && strict₂) p ε α) where
   hOrElse := hOrElse
 
 @[inline]
-instance {strict : Bool} {p : ValidPos s} {ε α} : OrElse (Result strict p ε α) where
+instance {strict : Bool} {p : Pos s} {ε α} : OrElse (Result strict p ε α) where
   orElse := orElse
 
 @[inline]
-instance {strict : Bool} {p : ValidPos s} {ε} : MonadExceptOf ε (Result strict p ε) where
+instance {strict : Bool} {p : Pos s} {ε} : MonadExceptOf ε (Result strict p ε) where
   throw := throw
   tryCatch := tryCatch
 
 @[inline]
-instance {strict : Bool} {p : ValidPos s} {ε} : Bind (Result strict p ε) where
+instance {strict : Bool} {p : Pos s} {ε} : Bind (Result strict p ε) where
   bind := bind
 
 @[inline]
-instance {p : ValidPos s} {ε} : Pure (LE p ε) where
+instance {p : Pos s} {ε} : Pure (LE p ε) where
   pure := pure
 
 @[inline]
-instance {p : ValidPos s} {ε} : Monad (LE p ε) where
+instance {p : Pos s} {ε} : Monad (LE p ε) where
   bind := bind
 
 end Result
